Progress on laying down the ground for I2F refinement. Need to take some time to do things cleanly for dependent inversions, it's a mess right now

src/rocq/Theory/I2F.v
@@ -1,7 +1,7 @@
 From ITree Require Import ITree Eq Rutt HeterogeneousRelations.
 
 From Vellvm Require Import
-  Utilities
+  Utils
   Syntax
   Integers
   DynamicValues
@@ -19,17 +19,42 @@ From Vellvm Require Import
 From Vellvm Require Import
   Theory.rutt_cutoff.
 
+From Paco Require Import paco.
+
+Definition sum_prerel {E1 E2 D1 D2 : Type -> Type} (PR1 : prerel E1 D1 ) (PR2 : prerel E2 D2) 
+  : prerel (E1 +' E2) (D1 +' D2) :=
+  fun A B e1 e2 =>
+    match e1,e2 with
+    | inl1 e1, inl1 e2 => PR1 _ _ e1 e2
+    | inr1 e1, inr1 e2 => PR2 _ _ e1 e2
+    | _,_ => False
+    end
+.
+
+Definition sum_postrel {E1 E2 D1 D2 : Type -> Type} (PR1 : postrel E1 D1 ) (PR2 : postrel E2 D2) 
+  : postrel (E1 +' E2) (D1 +' D2) :=
+  fun A B e1 a e2 b => 
+    match e1,e2 with
+    | inl1 e1, inl1 e2 => PR1 _ _ e1 a e2 b
+    | inr1 e1, inr1 e2 => PR2 _ _ e1 a e2 b
+    | _,_ => False
+    end
+.
+
+
 Section Refinement.
-  
+
   Definition PInf : Params := @ParamsV IPZ IPZTheory.
   Definition PFin : Params := @ParamsV IP64Bit IP64BitTheory.
+
+  (** * Value relations *)
 
   Definition I2F_Iptr : @iptr IPZ -> @iptr IP64Bit -> Prop :=
     fun z i => z = unsigned i.
 
   Definition I2F_Addr : @addr ProvenanceV (@AddressV IPZ) -> @addr ProvenanceV (@AddressV IP64Bit) -> Prop :=
     fun '(z,p) '(i,p') => I2F_Iptr z i /\ p = p'.
-  
+
   Inductive I2F_dvalue : @dvalue PInf -> @dvalue PFin -> Prop :=
   | I2F_dvalue_Addr a a' :
     I2F_Addr a a' ->
@@ -61,61 +86,337 @@ Section Refinement.
     I2F_dvalue (DVALUE_Vector τ s1) (DVALUE_Vector τ s2)
   .
 
-  Variant I2FE : forall A B, @CFGEtop PInf A -> @CFGEtop PFin B -> Prop :=
-    | I2FE_call τ dv1 args1 dv2 args2 :
-      I2F_dvalue dv1 dv2 ->
+  (* Exceptions are dvalues, and calls/intrinsics answer in [exc + dvalue] *)
+  Notation I2F_exc_dvalue := (sum_rel I2F_dvalue I2F_dvalue).
+
+  (** * Event relations, one per event family
+
+      Two events are related when they are the same constructor, carrying
+      pointwise [I2F]-related payloads. Recall the components that do not
+      mention values ([raw_id], [dtyp], intrinsic names, [int8] streams,
+      the [unit] messages of the abortive events) are shared between the
+      two instantiations, hence required equal. *)
+
+  Variant I2FE_Call : prerel (@CallE PInf) (@CallE PFin) :=
+    | I2FE_call τ f1 args1 f2 args2 :
+      I2F_dvalue f1 f2 ->
       Forall2 I2F_dvalue args1 args2 ->
-      I2FE (subevent _ (@Call PInf τ dv1 args1)) (subevent _ (@Call PFin τ dv2 args2))
-    | I2FE_extcall τ dv1 args1 dv2 args2 :
-      I2F_dvalue dv1 dv2 ->
+      I2FE_Call (@Call PInf τ f1 args1) (@Call PFin τ f2 args2)
+  .
+
+  Variant I2FE_ExternalCall : prerel (@ExternalCallE PInf) (@ExternalCallE PFin) :=
+    | I2FE_extcall τ f1 args1 f2 args2 :
+      I2F_dvalue f1 f2 ->
       Forall2 I2F_dvalue args1 args2 ->
-      I2FE (subevent _ (@ExternalCall PInf τ dv1 args1)) (subevent _ (@ExternalCall PFin τ dv2 args2))
-    | I2FE_stdout args :
-      I2FE (subevent _ (@IO_stdout PInf args)) (subevent _ (@IO_stdout PFin args))
-    | I2FE_stderr args :
-      I2FE (subevent _ (@IO_stderr PInf args)) (subevent _ (@IO_stderr PFin args))
-    | I2FE_intrinsic τ msg args1 oa1 args2 oa2 :
-      option_rel I2F_Addr oa1 oa2 ->
+      I2FE_ExternalCall (@ExternalCall PInf τ f1 args1) (@ExternalCall PFin τ f2 args2)
+    | I2FE_stdout str :
+      I2FE_ExternalCall (@IO_stdout PInf str) (@IO_stdout PFin str)
+    | I2FE_stderr str :
+      I2FE_ExternalCall (@IO_stderr PInf str) (@IO_stderr PFin str)
+  .
+
+  Variant I2FE_Intrinsic : prerel (@IntrinsicE PInf) (@IntrinsicE PFin) :=
+    | I2FE_intrinsic τ f args1 va1 args2 va2 :
       Forall2 I2F_dvalue args1 args2 ->
-      I2FE (subevent _ (@Intrinsic PInf τ msg args1 oa1)) (subevent _ (@Intrinsic PFin τ msg args2 oa2))
+      option_rel I2F_Addr va1 va2 ->
+      I2FE_Intrinsic (@Intrinsic PInf τ f args1 va1) (@Intrinsic PFin τ f args2 va2)
+  .
+
+  Variant I2FE_Global : prerel (@GlobalE PInf) (@GlobalE PFin) :=
     | I2FE_gwrite x dv1 dv2 :
       I2F_dvalue dv1 dv2 ->
-      I2FE (subevent _ (@GlobalWrite PInf x dv1)) (subevent _ (@GlobalWrite PFin x dv2))
+      I2FE_Global (@GlobalWrite PInf x dv1) (@GlobalWrite PFin x dv2)
     | I2FE_gread x :
-      I2FE (subevent _ (@GlobalRead PInf x)) (subevent _ (@GlobalRead PFin x))
+      I2FE_Global (@GlobalRead PInf x) (@GlobalRead PFin x)
+  .
+
+  Variant I2FE_Local : prerel (@LocalE PInf) (@LocalE PFin) :=
     | I2FE_lwrite x dv1 dv2 :
       I2F_dvalue dv1 dv2 ->
-      I2FE (subevent _ (@LocalWrite PInf x dv1)) (subevent _ (@LocalWrite PFin x dv2))
+      I2FE_Local (@LocalWrite PInf x dv1) (@LocalWrite PFin x dv2)
     | I2FE_lread x :
-      I2FE (subevent _ (@LocalRead PInf x)) (subevent _ (@LocalRead PFin x))
+      I2FE_Local (@LocalRead PInf x) (@LocalRead PFin x)
+  .
+
+  Variant I2FE_Stack : prerel (@StackE PInf) (@StackE PFin) :=
     | I2FE_spush args1 args2 :
       Forall2 (prod_rel Logic.eq I2F_dvalue) args1 args2 ->
-      I2FE (subevent _ (@StackPush PInf args1)) (subevent _ (@StackPush PFin args2))
+      I2FE_Stack (@StackPush PInf args1) (@StackPush PFin args2)
     | I2FE_spop :
-      I2FE (subevent _ (@StackPop PInf)) (subevent _ (@StackPop PFin))
-    | I2FE_ssethandler ob :
-      I2FE (subevent _ (@StackSetHandler PInf ob)) (subevent _ (@StackSetHandler PFin ob))
-    | I2FE_shandler :
-      I2FE (subevent _ (@StackHandler PInf)) (subevent _ (@StackHandler PFin))
+      I2FE_Stack (@StackPop PInf) (@StackPop PFin)
     | I2FE_sraise exc1 exc2 :
       I2F_dvalue exc1 exc2 ->
-      I2FE (subevent _ (@StackRaise PInf exc1)) (subevent _ (@StackRaise PFin exc2))
+      I2FE_Stack (@StackRaise PInf exc1) (@StackRaise PFin exc2)
     | I2FE_sgetexc :
-      I2FE (subevent _ (@StackGetExc PInf)) (subevent _ (@StackGetExc PFin))
-   .
-     
+      I2FE_Stack (@StackGetExc PInf) (@StackGetExc PFin)
+  .
+
+  Variant I2FE_Memory : prerel (@MemoryE PInf) (@MemoryE PFin) :=
+    | I2FE_mempush :
+      I2FE_Memory (@MemPush PInf) (@MemPush PFin)
+    | I2FE_mempop :
+      I2FE_Memory (@MemPop PInf) (@MemPop PFin)
+    | I2FE_alloca τ n align :
+      I2FE_Memory (@Alloca PInf τ n align) (@Alloca PFin τ n align)
+    | I2FE_load τ a1 a2 :
+      I2F_dvalue a1 a2 ->
+      I2FE_Memory (@Load PInf τ a1) (@Load PFin τ a2)
+    | I2FE_store τ a1 v1 a2 v2 :
+      I2F_dvalue a1 a2 ->
+      I2F_dvalue v1 v2 ->
+      I2FE_Memory (@Store PInf τ a1 v1) (@Store PFin τ a2 v2)
+  .
+
+  Variant I2FE_Draw : prerel (@DrawE PInf) (@DrawE PFin) :=
+    | I2FE_draw τ :
+      I2FE_Draw (@Draw PInf τ) (@Draw PFin τ)
+  .
+
+  Variant I2FE_Exc : prerel (@LLVMExcE PInf) (@LLVMExcE PFin) :=
+    | I2FE_exc exc1 exc2 :
+      I2F_dvalue exc1 exc2 ->
+      I2FE_Exc (@LLVMExc PInf exc1) (@LLVMExc PFin exc2)
+  .
+
+  (* [OOME], [UBE], [DebugE], [FailureE] do not mention values: they are
+     shared by both instantiations. Note that pairs of related [OOME]
+     (resp. [UBE]) events can alternatively be discharged by the cut
+     mechanism of [ruttc] --- see [I2F_refine] below. *)
+
+  Variant I2FE_OOM : prerel OOME OOME :=
+    | I2FE_throwOOM u1 u2 :
+      I2FE_OOM (ThrowOOM u1) (ThrowOOM u2)
+  .
+
+  Variant I2FE_UB : prerel UBE UBE :=
+    | I2FE_throwUB u1 u2 :
+      I2FE_UB (ThrowUB u1) (ThrowUB u2)
+  .
+
+  Variant I2FE_Debug : prerel DebugE DebugE :=
+    | I2FE_debug u1 u2 :
+      I2FE_Debug (Debug u1) (Debug u2)
+  .
+
+  Variant I2FE_Failure : prerel FailureE FailureE :=
+    | I2FE_throw u1 u2 :
+      I2FE_Failure (Throw u1) (Throw u2)
+  .
+
+  (** * Answer relations, one per event family
+
+      [ruttc] additionally takes a relation on the answers returned to two
+      related events: when relating [Vis e1 k1] with [Vis e2 k2], the
+      continuations only have to be related on pairs of answers related by
+      it. It is our relational assumption on the environment, to be
+      discharged when interpreting each event family: the answers are
+      related by the [I2F] value relation matching the answer type of the
+      event --- [I2F_dvalue] on [dvalue] answers, its [sum_rel]
+      (resp. [option_rel]) lifting on [exc + dvalue] (resp. [option exc])
+      answers, trivial on [unit], and vacuous on [void] (abortive events
+      never answer). *)
+
+  Variant I2FA_Call : postrel (@CallE PInf) (@CallE PFin) :=
+    | I2FA_call τ1 f1 args1 τ2 f2 args2 r1 r2 :
+      I2F_exc_dvalue r1 r2 ->
+      I2FA_Call (@Call PInf τ1 f1 args1) r1 (@Call PFin τ2 f2 args2) r2
+  .
+
+  Variant I2FA_ExternalCall : postrel (@ExternalCallE PInf) (@ExternalCallE PFin) :=
+    | I2FA_extcall τ1 f1 args1 τ2 f2 args2 dv1 dv2 :
+      I2F_dvalue dv1 dv2 ->
+      I2FA_ExternalCall (@ExternalCall PInf τ1 f1 args1) dv1 (@ExternalCall PFin τ2 f2 args2) dv2
+    | I2FA_stdout str1 str2 (a b : unit) :
+      I2FA_ExternalCall (@IO_stdout PInf str1) a (@IO_stdout PFin str2) b
+    | I2FA_stderr str1 str2 (a b : unit) :
+      I2FA_ExternalCall (@IO_stderr PInf str1) a (@IO_stderr PFin str2) b
+  .
+
+  Variant I2FA_Intrinsic : postrel (@IntrinsicE PInf) (@IntrinsicE PFin) :=
+    | I2FA_intrinsic τ1 f1 args1 va1 τ2 f2 args2 va2 r1 r2 :
+      I2F_exc_dvalue r1 r2 ->
+      I2FA_Intrinsic (@Intrinsic PInf τ1 f1 args1 va1) r1 (@Intrinsic PFin τ2 f2 args2 va2) r2
+  .
+
+  Variant I2FA_Global : postrel (@GlobalE PInf) (@GlobalE PFin) :=
+    | I2FA_gwrite x1 dv1 x2 dv2 (a b : unit) :
+      I2FA_Global (@GlobalWrite PInf x1 dv1) a (@GlobalWrite PFin x2 dv2) b
+    | I2FA_gread x1 x2 dv1 dv2 :
+      I2F_dvalue dv1 dv2 ->
+      I2FA_Global (@GlobalRead PInf x1) dv1 (@GlobalRead PFin x2) dv2
+  .
+
+  Variant I2FA_Local : postrel (@LocalE PInf) (@LocalE PFin) :=
+    | I2FA_lwrite x1 dv1 x2 dv2 (a b : unit) :
+      I2FA_Local (@LocalWrite PInf x1 dv1) a (@LocalWrite PFin x2 dv2) b
+    | I2FA_lread x1 x2 dv1 dv2 :
+      I2F_dvalue dv1 dv2 ->
+      I2FA_Local (@LocalRead PInf x1) dv1 (@LocalRead PFin x2) dv2
+  .
+
+  Variant I2FA_Stack : postrel (@StackE PInf) (@StackE PFin) :=
+    | I2FA_spush args1 args2 (a b : unit) :
+      I2FA_Stack (@StackPush PInf args1) a (@StackPush PFin args2) b
+    | I2FA_spop (a b : unit) :
+      I2FA_Stack (@StackPop PInf) a (@StackPop PFin) b
+    | I2FA_sraise exc1 exc2 (a b : unit) :
+      I2FA_Stack (@StackRaise PInf exc1) a (@StackRaise PFin exc2) b
+    | I2FA_sgetexc oe1 oe2 :
+      option_rel I2F_dvalue oe1 oe2 ->
+      I2FA_Stack (@StackGetExc PInf) oe1 (@StackGetExc PFin) oe2
+  .
+
+  Variant I2FA_Memory : postrel (@MemoryE PInf) (@MemoryE PFin) :=
+    | I2FA_mempush (a b : unit) :
+      I2FA_Memory (@MemPush PInf) a (@MemPush PFin) b
+    | I2FA_mempop (a b : unit) :
+      I2FA_Memory (@MemPop PInf) a (@MemPop PFin) b
+    (* [Alloca] answers with the fresh address wrapped as a [dvalue]:
+       the two memories allocate at [I2F_Addr]-related addresses. *)
+    | I2FA_alloca τ1 n1 align1 τ2 n2 align2 dv1 dv2 :
+      I2F_dvalue dv1 dv2 ->
+      I2FA_Memory (@Alloca PInf τ1 n1 align1) dv1 (@Alloca PFin τ2 n2 align2) dv2
+    | I2FA_load τ1 a1 τ2 a2 dv1 dv2 :
+      I2F_dvalue dv1 dv2 ->
+      I2FA_Memory (@Load PInf τ1 a1) dv1 (@Load PFin τ2 a2) dv2
+    | I2FA_store τ1 a1 v1 τ2 a2 v2 (a b : unit) :
+      I2FA_Memory (@Store PInf τ1 a1 v1) a (@Store PFin τ2 a2 v2) b
+  .
+
+  Variant I2FA_Draw : postrel (@DrawE PInf) (@DrawE PFin) :=
+    | I2FA_draw τ1 τ2 dv1 dv2 :
+      I2F_dvalue dv1 dv2 ->
+      I2FA_Draw (@Draw PInf τ1) dv1 (@Draw PFin τ2) dv2
+  .
+
+  (* The abortive events answer in [void]: their answer relations are
+     vacuous, and so are the associated continuation proof obligations. *)
+
+  Variant I2FA_Exc : postrel (@LLVMExcE PInf) (@LLVMExcE PFin) :=
+    | I2FA_exc exc1 exc2 (a b : void) :
+      I2FA_Exc (@LLVMExc PInf exc1) a (@LLVMExc PFin exc2) b
+  .
+
+  Variant I2FA_OOM : postrel OOME OOME :=
+    | I2FA_throwOOM u1 u2 (a b : void) :
+      I2FA_OOM (ThrowOOM u1) a (ThrowOOM u2) b
+  .
+
+  Variant I2FA_UB : postrel UBE UBE :=
+    | I2FA_throwUB u1 u2 (a b : void) :
+      I2FA_UB (ThrowUB u1) a (ThrowUB u2) b
+  .
+
+  Variant I2FA_Debug : postrel DebugE DebugE :=
+    | I2FA_debug u1 u2 (a b : unit) :
+      I2FA_Debug (Debug u1) a (Debug u2) b
+  .
+
+  Variant I2FA_Failure : postrel FailureE FailureE :=
+    | I2FA_throw u1 u2 (a b : void) :
+      I2FA_Failure (Throw u1) a (Throw u2) b
+  .
+
+  (** * Combined relations on [MCFGEtop] and [CFGEtop]
+
+      The per-family relations are glued along the structure of the event
+      signatures with [sum_prerel]/[sum_postrel]. This is the format
+      expected by the [mrec] reasoning principle
+      ([RuttFacts.interp_mrec_rutt] and its [ruttc] analogue to come):
+      since [CFGEtop ≡ CallE +' MCFGEtop] and [denote_mcfg] is an [mrec]
+      over [CallE], the [CFG]-level relations are literally
+      [sum_prerel I2FE_Call I2FE_MCFG] / [sum_postrel I2FA_Call I2FA_MCFG]. *)
+
+  Definition I2FE_MCFG : prerel (@MCFGEtop PInf) (@MCFGEtop PFin) :=
+    sum_prerel I2FE_ExternalCall
+      (sum_prerel I2FE_Intrinsic
+         (sum_prerel I2FE_Global
+            (sum_prerel (sum_prerel I2FE_Local I2FE_Stack)
+               (sum_prerel I2FE_Memory
+                  (sum_prerel I2FE_Draw
+                     (sum_prerel I2FE_OOM
+                        (sum_prerel I2FE_Exc
+                           (sum_prerel I2FE_UB
+                              (sum_prerel I2FE_Debug I2FE_Failure))))))))).
+
+  Definition I2FA_MCFG : postrel (@MCFGEtop PInf) (@MCFGEtop PFin) :=
+    sum_postrel I2FA_ExternalCall
+      (sum_postrel I2FA_Intrinsic
+         (sum_postrel I2FA_Global
+            (sum_postrel (sum_postrel I2FA_Local I2FA_Stack)
+               (sum_postrel I2FA_Memory
+                  (sum_postrel I2FA_Draw
+                     (sum_postrel I2FA_OOM
+                        (sum_postrel I2FA_Exc
+                           (sum_postrel I2FA_UB
+                              (sum_postrel I2FA_Debug I2FA_Failure))))))))).
+
+  Definition I2FE_CFG : prerel (@CFGEtop PInf) (@CFGEtop PFin) :=
+    sum_prerel I2FE_Call I2FE_MCFG.
+
+  Definition I2FA_CFG : postrel (@CFGEtop PInf) (@CFGEtop PFin) :=
+    sum_postrel I2FA_Call I2FA_MCFG.
+
+  (** * The refinement relation *)
+
+  Variant cutUB {E} `{UBE -< E} : forall [A], E A -> Prop :=
+    | CutUB v : cutUB (subevent _ (ThrowUB v)).
+
+  Variant cutOOM {E} `{OOME -< E} : forall [A], E A -> Prop :=
+    | CutOOM v : cutOOM (subevent _ (ThrowOOM v)).
+
+  (* The infinite computation (left) and the finite one (right) proceed in
+     lockstep over [I2FE]-related events answered by [I2FA]-related values,
+     except that the equivalence is short-circuited if the finite side runs
+     out of memory (cut on OOM on the right); UB should arise simultaneously
+     on both sides, so we may cut it off on the left. *)
+
+  Definition I2F_refine_MCFG {R1 R2} (RR : R1 -> R2 -> Prop)
+    : @MCFGtop PInf R1 -> @MCFGtop PFin R2 -> Prop :=
+    ruttc cutUB cutOOM I2FE_MCFG I2FA_MCFG RR.
+
+  Definition I2F_refine_CFG {R1 R2} (RR : R1 -> R2 -> Prop)
+    : @CFGtop PInf R1 -> @CFGtop PFin R2 -> Prop :=
+    ruttc cutUB cutOOM I2FE_CFG I2FA_CFG RR.
+
+  Definition I2F_refine : @MCFGtop PInf (@dvalue PInf) -> @MCFGtop PFin (@dvalue PFin) -> Prop :=
+    I2F_refine_MCFG I2F_dvalue.
+
+(* Lemma I2F_refine_MCFG_trigger {A B} (e : @MCFGEtop PInf A) (f : @MCFGEtop PFin B) RR : *)
+(*   I2FE_MCFG e f -> *)
+(*   I2F_refine_MCFG RR (ITree.trigger e) (ITree.trigger f). *)
+(* Proof. *)
+(*   intros; apply ruttc_trigger; auto. *)
+   
+  Hint Constructors I2FA_Local.
+Require Import Stdlib.Program.Equality.
+  Lemma denote_expr :
+    forall (e : exp dtyp) τ, I2F_refine (@denote_exp PInf τ e) (@denote_exp PFin τ e).
+  Proof.
+    apply (@exp_ind dtyp (fun e => forall τ, I2F_refine (@denote_exp PInf τ e) (@denote_exp PFin τ e)) (fun _ => True)); auto.
+    - intros; cbn.
+      destruct id; cbn.
+      + apply ruttc_trigger.
+        constructor.
+        cbn.
+        intros.
+        dependent induction H; subst; auto.
+
+      apply I2F_refine_MCFG_trigger.
+    intros e.
+    induction e with (Q := fun _ => True).
 
   (* Lemma denote_ok : Prop. *)
-  (*   refine (forall i oa oa', rutt I2FE _ _ (@denote_instr PInf i oa) (@denote_instr PFin i (_ oa))). *)
+  (*   refine (forall i oa oa', rutt I2FE (@denote_instr PInf i oa) (@denote_instr PFin i (_ oa))). *)
   (*   3: refine (fmap _). *)
   (*   3: refine (fun '(a,p) => _). *)
   (*  3:{ cbn. *)
-    
-  
+
+
   (* Lemma handle_memory_refine : Prop. *)
   (*   refine (forall {X} (e : @MemoryE PInf X), _ : Prop). *)
   (*     @handle_memoryM PIn *)
 
 
- 
+
 End Refinement.
